document + clean

theories/LevelTwoClean.v
@@ -2,24 +2,23 @@ From Prototype Require Import Prelude Sig LevelTwo.
 From Prototype Require LevelOne.
 Module O := LevelOne.
 
-
 (** The output of simplification (LevelTwoSimp.v) is good for comparing
     terms/equations for equality, but not very nice to work with. 
     This file implements cleanup functions which do trivial transformations 
-    such as turning [Q_rapply R_shift i] into [Q_succ i]. Cleanup is
-    typically applied after simplification.
-
-    Cleanup functions can be applied to all terms (irreducible or not),
-    and do not produce irreducible terms.
+    such as turning [Q_rapply R_shift i] into [Q_succ i], and are 
+    typically applied after simplification. Cleanup functions can be applied to all terms (not only the output 
+    of [LevelTwoSimp.v].
     
-    For each cleanup function we prove a soundness lemma. *)
+    We formulate the correctness of cleanup as a rewriting system 
+    ([qred], [rred], [ered], [sred]), which is proved correct with 
+    respect to evaluation (lemmas [ered_sound], [sred_sound], etc).
+    Contrary to simplification, we don't prove that we obtain
+    irreducible forms (for the cleanup rewriting system), although
+    we conjecture that it is true.  *)
 
 Section WithSignature.
 Context {sig : signature}.
 #[local] Existing Instance sig.
-
-(** Add some power to [auto] and variants (such as [triv]). *)
-#[local] Hint Extern 5 => intros ? : core.
 
 (*********************************************************************************)
 (** *** [mk_qsucc] *)
@@ -54,7 +53,7 @@ Lemma nat_add_spec n m : nat_add n m = n + m.
 Proof. funelim (nat_add n m) ; triv. rewrite H. lia. Qed. 
 
 (** [dest_rshift r] checks if [r] is of the form [rshift >> rshift >> rshift >> ...]
-    (with at least one shift): 
+    (with at least one shift, and up to associativity): 
     - if so it returns [Some n] where [S n] is the number of shifts.
     - otherwise it returns [None]. *)
 Equations dest_rshift (r : ren) : option nat :=
@@ -255,211 +254,19 @@ Lemma sred_sound e s s' : s =s=> s' -> seval e s =₁ seval e s'.
 Proof. now apply ered_sred_sound. Qed.
 
 (*********************************************************************************)
-(** *** Irreducible & reducible forms. *)
-(*********************************************************************************)
-
-(** The "true" definition of irreducible forms, i.e. terms in which we can't 
-    reduce. This definition is obviously correct but is hard to work with. *)
-Definition qirred i := forall i', i =q=> i' -> i = i'.
-Definition rirred r := forall r', r =r=> r' -> r = r'.
-Definition eirred {k} (t : expr k) := forall t', t =e=> t' -> t = t'.
-Definition sirred s := forall s', s =s=> s' -> s = s'.
-
-Unset Elimination Schemes.
-
-(** A definition of reducible forms, i.e. terms in which we can reduce,
-    which is easy to work with but is not obviously correct.
-    We prove below that this notion agrees with [qirred], [rirred], etc. *)
-Inductive qreducible : qnat -> Prop :=
-(* Congruence. *)
-| qreducible_congr_succ i : qreducible i -> qreducible (Q_succ i)
-| qreducible_congr_rapply_1 r i : rreducible r -> qreducible (Q_rapply r i)
-| qreducible_congr_rapply_2 r i : qreducible i -> qreducible (Q_rapply r i)
-(* Cleanup rules. *)
-| qreducible_rapply_shift r i n : dest_rshift r = Some n -> qreducible (Q_rapply r i)
-
-with rreducible : ren -> Prop :=
-(* Congruence. *)
-| rreducible_congr_cons_1 i r : qreducible i -> rreducible (R_cons i r)
-| rreducible_congr_cons_2 i r : rreducible r -> rreducible (R_cons i r)
-| rreducible_congr_comp_1 r1 r2 : rreducible r1 -> rreducible (R_comp r1 r2)
-| rreducible_congr_comp_2 r1 r2 : rreducible r2 -> rreducible (R_comp r1 r2).
-
-Inductive ereducible : forall {k}, expr k -> Prop :=
-(* Congruence. *)
-| ereducible_congr_tvar i : qreducible i -> ereducible (E_tvar i)
-| ereducible_congr_tctor c al : ereducible al -> ereducible (E_tctor c al)
-| ereducible_congr_al_cons_1 {ty tys} (a : expr (Ka ty)) (al : expr (Kal tys)) : 
-    ereducible a -> ereducible (E_al_cons a al)
-| ereducible_congr_al_cons_2 {ty tys} (a : expr (Ka ty)) (al : expr (Kal tys)) : 
-    ereducible al -> ereducible (E_al_cons a al)
-| ereducible_congr_aterm t : ereducible t -> ereducible (E_aterm t)
-| ereducible_congr_abind {ty} (a : expr (Ka ty)) : ereducible a -> ereducible (E_abind a)
-| ereducible_congr_ren_1 {k} r (t : expr k) : rreducible r -> ereducible (E_ren r t)
-| ereducible_congr_ren_2 {k} r (t : expr k) : ereducible t -> ereducible (E_ren r t)
-| ereducible_congr_subst_1 {k} s (t : expr k) : sreducible s -> ereducible (E_subst s t)
-| ereducible_congr_subst_2 {k} s (t : expr k) : ereducible t -> ereducible (E_subst s t)
-(* Cleanup rules. *)
-| ereducible_ren_var r i : ereducible (E_ren r (E_tvar i))
-| ereducible_subst_ren {k} s r (t : expr k) : dest_ren s = Some r -> ereducible (E_subst s t)
-
-with sreducible : subst -> Prop :=
-(* Congruence. *)
-| sreducible_congr_cons_1 t s : ereducible t -> sreducible (S_cons t s)
-| sreducible_congr_cons_2 t s : sreducible s -> sreducible (S_cons t s)
-| sreducible_congr_comp_1 s1 s2 : sreducible s1 -> sreducible (S_comp s1 s2)
-| sreducible_congr_comp_2 s1 s2 : sreducible s2 -> sreducible (S_comp s1 s2)
-| sreducible_congr_ren r : rreducible r -> sreducible (S_ren r).
-
-Set Elimination Schemes.
-
-Scheme qreducible_ind := Minimality for qreducible Sort Prop 
-  with rreducible_ind := Minimality for rreducible Sort Prop.
-Combined Scheme qreducible_rreducible_ind from qreducible_ind, rreducible_ind.
-
-Scheme ereducible_ind := Minimality for ereducible Sort Prop 
-  with sreducible_ind := Minimality for sreducible Sort Prop.
-Combined Scheme ereducible_sreducible_ind from ereducible_ind, sreducible_ind.
-
-Derive Signature for qreducible rreducible ereducible sreducible.
-
-#[local] Hint Constructors qreducible rreducible ereducible sreducible : core.
-
-(*********************************************************************************)
-(** *** Equivalence between the two notions of irreducible forms. *)
-(*********************************************************************************)
-
-Lemma qr_red_impl_reducible : 
-  (forall i i', i =q=> i' -> i = i' \/ qreducible i) /\ 
-  (forall r r', r =r=> r' -> r = r' \/ rreducible r).
-Proof.
-apply qred_rred_ind ; intros ; triv.
-all: try solve [ destruct H0, H2 ; triv ].
-destruct H0 ; triv.
-Qed.
-
-Lemma qr_reducible_impl_red : 
-  (forall i, qreducible i -> exists i', i =q=> i' /\ i <> i') /\
-  (forall r, rreducible r -> exists r', r =r=> r' /\ r <> r').
-Proof.
-apply qreducible_rreducible_ind ; intros.
-all: try solve [ destruct H0 as (i' & H1 & H2) ; eexists ; split ; 
-  [now rewrite H1 | intros H3 ; now depelim H3] ].
-exists (mk_qsucc n i). split ; triv. destruct n ; triv.
-Qed.
-
-Lemma es_red_impl_reducible : 
-  (forall {k} (t t' : expr k), t =e=> t' -> t = t' \/ ereducible t) /\ 
-  (forall s s', s =s=> s' -> s = s' \/ sreducible s).
-Proof.
-apply ered_sred_ind ; intros ; triv.
-all: try solve [ destruct H0 ; triv | destruct H0, H2 ; triv ].
-- apply qr_red_impl_reducible in H. destruct H ; triv.
-- apply qr_red_impl_reducible in H. destruct H, H1 ; triv.
-- apply qr_red_impl_reducible in H. destruct H ; triv.   
-Qed.
-
-Lemma es_reducible_impl_red : 
-  (forall {k} (t : expr k), ereducible t -> exists t', t =e=> t' /\ t <> t') /\
-  (forall s, sreducible s -> exists s', s =s=> s' /\ s <> s').
-Proof.
-apply ereducible_sreducible_ind ; intros.
-all: try solve [ destruct H0 as (i' & H1 & H2) ; eexists ; split ; 
-  [now rewrite H1 | intros H3 ; now depelim H3] ].
-all: try solve [ apply qr_reducible_impl_red in H ; destruct H as (i' & H1 & H2) ;
-  eexists ; split ; [now rewrite H1 | intros H3 ; now depelim H3] ].
-- destruct H0 as (i' & H1 & H2). eexists.
-  split ; [now rewrite H1 | intros H3]. admit.
-- exists (E_tvar (Q_rapply r i)). triv.
-- exists (E_ren r t). split ; auto using ered_subst_ren. intros H1. depelim H1.
-Admitted.
-
-Lemma qirred_qreducible i : qirred i <-> ~qreducible i.
-Proof.
-split.
-- intros H H'. apply qr_reducible_impl_red in H'. destruct H' as (i' & H1 & H2). triv.
-- intros H i' Hi. apply qr_red_impl_reducible in Hi. destruct Hi ; triv.
-Qed.
-
-Lemma rirred_rreducible r : rirred r <-> ~rreducible r.
-Proof.
-split.
-- intros H H'. apply qr_reducible_impl_red in H'. destruct H' as (r' & H1 & H2). triv.
-- intros H r' Hr. apply qr_red_impl_reducible in Hr. destruct Hr ; triv.
-Qed.
-
-Lemma eirred_ereducible {k} (t : expr k) : eirred t <-> ~ereducible t.
-Proof.
-split.
-- intros H H'. apply es_reducible_impl_red in H'. destruct H' as (t' & H1 & H2). triv.
-- intros H t' Ht. apply es_red_impl_reducible in Ht. destruct Ht ; triv.
-Qed.
-
-Lemma sirred_sreducible s : sirred s <-> ~sreducible s.
-Proof.
-split.
-- intros H H'. apply es_reducible_impl_red in H'. destruct H' as (s' & H1 & H2). triv.
-- intros H s' Hs. apply es_red_impl_reducible in Hs. destruct Hs ; triv.
-Qed.
-
-(*********************************************************************************)
-(** *** Characterization of irreducible forms. *)
-(*********************************************************************************)
-
-Lemma qirred_succ i : qirred (Q_succ i) <-> qirred i.
-Proof.
-repeat rewrite qirred_qreducible.
-split ; intros H H1 ; apply H ; clear H ; triv. now depelim H1.
-Qed.
-
-Lemma qirred_rapply r i :
-  qirred (Q_rapply r i) <-> rirred r /\ qirred i /\ dest_rshift r = None.
-Proof.
-repeat rewrite rirred_rreducible ; repeat rewrite qirred_qreducible. split ; intros H.
-- split3 ; triv. destruct (dest_rshift r) eqn:E ; triv. exfalso. triv.
-- intros H'. depelim H' ; triv. rewrite H0 in H ; triv.
-Qed.
-
-Lemma rirred_cons i r : 
-  rirred (R_cons i r) <-> qirred i /\ rirred r.
-Proof.
-repeat rewrite rirred_rreducible ; repeat rewrite qirred_qreducible. 
-split ; intros H.
-- split ; triv.
-- intros H'. depelim H' ; triv.
-Qed.
-
-Lemma rirred_comp r1 r2 : 
-  rirred (R_comp r1 r2) <-> rirred r1 /\ rirred r2.
-Proof.
-repeat rewrite rirred_rreducible. split ; intros H.
-- split ; triv.
-- intros H'. depelim H' ; triv.
-Qed.  
-
-(*********************************************************************************)
-(** *** [clean_rapply]. *)
+(** *** [rapply]. *)
 (*********************************************************************************)
 
 (** Cleanup [Q_rapply r i]. *)
-Equations clean_rapply : ren -> qnat -> qnat :=
-clean_rapply r i with dest_rshift r := { 
+Equations rapply : ren -> qnat -> qnat :=
+rapply r i with dest_rshift r := { 
   | Some n => mk_qsucc n i 
   | None => Q_rapply r i
   }. 
 
-Lemma clean_rapply_red r i : 
-  Q_rapply r i =q=> clean_rapply r i.
-Proof. funelim (clean_rapply r i) ; triv. Qed.
-#[local] Hint Rewrite <-clean_rapply_red : red.
-
-Lemma clean_rapply_irred r i :
-  rirred r -> qirred i -> qirred (clean_rapply r i).
-Proof.
-intros H1 H2. funelim (clean_rapply r i).
-- induction n in |- * ; simp mk_qsucc ; now rewrite qirred_succ.
-- rewrite qirred_rapply. triv.
-Qed.
+Lemma rapply_red r i : Q_rapply r i =q=> rapply r i.
+Proof. funelim (rapply r i) ; triv. Qed.
+#[local] Hint Rewrite <-rapply_red : red.
 
 (*********************************************************************************)
 (** *** [qclean] and [rclean]. *)
@@ -468,7 +275,7 @@ Qed.
 Equations qclean : qnat -> qnat :=
 qclean Q_zero := Q_zero ;
 qclean (Q_succ i) := Q_succ (qclean i) ;
-qclean (Q_rapply r i) := clean_rapply (rclean r) (qclean i) ;
+qclean (Q_rapply r i) := rapply (rclean r) (qclean i) ;
 qclean (Q_mvar m) := Q_mvar m
 
 with rclean : ren -> ren :=
@@ -485,9 +292,7 @@ apply qclean_elim with
   (P := fun i res => i =q=> res)
   (P0 := fun r res => r =r=> res).
 all: intros ; simp red ; triv.
-- now rewrite <-H, <-H0.
-- now rewrite <-H, <-H0.
-- now rewrite <-H, <-H0.
+all: solve [ now rewrite <-H, <-H0 ].
 Qed.
 
 Lemma qclean_red i : i =q=> qclean i.
@@ -499,34 +304,32 @@ Proof. now apply qrclean_red. Qed.
 #[local] Hint Rewrite <-rclean_red : red.
 
 (*********************************************************************************)
-(** *** [clean_rename] *)
+(** *** [rename] *)
 (*********************************************************************************)
 
 (** Cleanup [E_ren r t]. *)
-Equations clean_rename {k} : ren -> expr k -> expr k :=
-clean_rename r (E_tvar i) := E_tvar (clean_rapply r i) ;
-clean_rename r t := E_ren r t.
+Equations rename {k} : ren -> expr k -> expr k :=
+rename r (E_tvar i) := E_tvar (rapply r i) ;
+rename r t := E_ren r t.
 
-Lemma clean_rename_red {k} r (t : expr k) :
-  E_ren r t =e=> clean_rename r t.
-Proof. funelim (clean_rename r t) ; simp red ; triv. Qed.
-#[local] Hint Rewrite <-@clean_rename_red : red.
+Lemma rename_red {k} r (t : expr k) : E_ren r t =e=> rename r t.
+Proof. funelim (rename r t) ; simp red ; triv. Qed.
+#[local] Hint Rewrite <-@rename_red : red.
 
 (*********************************************************************************)
-(** *** [clean_substitute] *)
+(** *** [substitute] *)
 (*********************************************************************************)
 
 (** Cleanup [E_subst s t]. *)
-Equations clean_substitute {k} : subst -> expr k -> expr k :=
-clean_substitute s t with dest_ren s := {
-  | Some r => clean_rename r t 
+Equations substitute {k} : subst -> expr k -> expr k :=
+substitute s t with dest_ren s := {
+  | Some r => rename r t 
   | None => E_subst s t
   }.
 
-Lemma clean_substitute_red {k} s (t : expr k) : 
-  E_subst s t =e=> clean_substitute s t.
-Proof. funelim (clean_substitute s t) ; simp red ; triv. Qed.
-#[local] Hint Rewrite <-@clean_substitute_red : red.
+Lemma substitute_red {k} s (t : expr k) : E_subst s t =e=> substitute s t.
+Proof. funelim (substitute s t) ; simp red ; triv. Qed.
+#[local] Hint Rewrite <-@substitute_red : red.
 
 (*********************************************************************************)
 (** *** [eclean] and [sclean] *)
@@ -540,8 +343,8 @@ eclean (E_al_cons a al) := E_al_cons (eclean a) (eclean al) ;
 eclean (E_abase b x) := E_abase b x ;
 eclean (E_aterm t) := E_aterm (eclean t) ;
 eclean (E_abind a) := E_abind (eclean a) ;
-eclean (E_ren r t) := clean_rename (rclean r) (eclean t) ;
-eclean (E_subst s t) := clean_substitute (sclean s) (eclean t) ;
+eclean (E_ren r t) := rename (rclean r) (eclean t) ;
+eclean (E_subst s t) := substitute (sclean s) (eclean t) ;
 eclean (E_mvar m) := E_mvar m
 
 with sclean : subst -> subst :=
@@ -552,9 +355,8 @@ sclean (S_comp s1 s2) := S_comp (sclean s1) (sclean s2) ;
 sclean (S_ren r) := S_ren (rclean r) ;
 sclean (S_mvar m) := S_mvar m.
 
-Lemma eclean_subst_red : 
-  (forall k (t : expr k), t =e=> eclean t) *
-  (forall s, s =s=> sclean s).
+Lemma eclean_sclean_red : 
+  (forall k (t : expr k), t =e=> eclean t) * (forall s, s =s=> sclean s).
 Proof.
 apply eclean_elim with 
   (P := fun k t res => t =e=> res) 
@@ -564,11 +366,11 @@ all: solve [ now rewrite <-H | now rewrite <-H, <-H0 ].
 Qed. 
 
 Lemma eclean_red {k} (t : expr k) : t =e=> eclean t.
-Proof. now apply eclean_subst_red. Qed.
+Proof. now apply eclean_sclean_red. Qed.
 #[local] Hint Rewrite @eclean_red : red.
 
 Lemma sclean_red s : s =s=> sclean s.
-Proof. now apply eclean_subst_red. Qed.
+Proof. now apply eclean_sclean_red. Qed.
 #[local] Hint Rewrite sclean_red : red.
 
 End WithSignature.
